Proofreading and minor style

Manual/RecursiveDefs/PartialFixpoint.lean
@@ -16,38 +16,54 @@ open Lean.Elab.Tactic.GuardMsgs.WhitespaceMode
 
 open Lean.Order
 
+set_option maxRecDepth 600
+
 #doc (Manual) "Partial Fixpoint Recursion" =>
 %%%
 tag := "partial-fixpoint"
 %%%
 
-A function definition can be understood as a request to Lean to construct a function of the given type that satisfies the given equation.
-One purpose of the termination proof in {ref "structural-recursion"}[structural recursion] or {ref "well-founded-recursion"}[well-founded recursion] is to guarantee the existence and uniqueness the constructed functions.
+All definitions are fundamentally equations: the new constant being defined is equal to the right-hand side of the definition.
+For functions defined by {ref "structural-recursion"}[structural recursion], this equation holds {tech key:="definitional equality"}[definitionally], and there is a unique value returned by application of the function.
+For functions defined by {ref "well-founded-recursion"}[well-founded recursion], the equation may hold only {tech key:="proposition"}[propositionally], but all type-correct applications of the function to arguments are equal to the respective values prescribed by the definition.
+In both cases, the fact that the function terminates for all inputs means that the value computed by applying the function is always uniquely determined.
 
-In some cases, the equation may not uniquely determine the function's (extensional) behavior, because it
-does not terminate for all arguments in the above sense, but there still exist functions for which the defining equation holds.
-In these cases, a definition by {deftech}_partial fixpoint_ may be possible.
 
-Even in cases where the defining equation fully describes the function's behavior and a termination proof using {ref "well-founded-recursion"}[well-founded recursion] would be possible it may simply be more convenient to define the function using partial fixpoint, to avoid a possible tedious termination proof.
+In some cases where a function does not terminate for all arguments, the equation may not uniquely determine the function's return value for each input, but there are nonetheless functions for which the defining equation holds.
+In these cases, a definition as a {deftech}_partial fixpoint_ may still be possible.
+Any function that satisfies the defining equation can be used to demonstrate that the equation does not create a logical contradiction, and the equation can then be proven as a theorem about this function.
+As with the other strategies for defining recursive functions, compiled code uses the function as it was originally written; like definitions in terms of eliminators or recursion over accessibility proofs, the function used to define the partial fixpoint is used only to justify the function's equations in Lean's logic for purposes of mathematical reasoning.
 
-Definition by partial fixpoint is only used when explicitly requested by the user, by annotating the definition with {keywordOf Lean.Parser.Command.declaration}`partial_fixpoint`.
+While partial fixpoints do allow more funtions to be defined in Lean, the are also useful for functions that can be defined without them.
+Even in cases where the defining equation fully describes the function's behavior and a termination proof using {ref "well-founded-recursion"}[well-founded recursion] would be possible, it may simply be more convenient to define the function as a partial fixpoint to avoid a having to write a termination proof.
 
-There are two classes of functions for which a definition by partial fixpoint works:
+Defining recursive functions as partial fixpoints only occurs when explicitly requested by annotating the definition with {keywordOf Lean.Parser.Command.declaration}`partial_fixpoint`.
 
-* tail-recursive functions of inhabited type, and
-* monadic functions in a suitable monad, such as the {name}`Option` monad.
+:::paragraph
+There are two classes of functions that can be defined as partial fixpoints:
+
+ * Tail-recursive functions whose return type is inhabited type
+
+ * Functions that return values in a suitable monad, such as the {name}`Option` monad
 
 Both classes are backed by the same theory and construction: least fixpoints of monotone equations in chain-complete partial orders.
 
-Lean supports {tech}[mutually recursive] functions to be defined by partial fixpoint.
-For this, every function definition in a mutual block has to be annotated with {keywordOf Lean.Parser.Command.declaration}`partial_fixpoint`.
+:::
+
+Just as with structural and well-founded recursion, Lean allows {tech}[mutually recursive] functions to be defined as partial fixpoints.
+To use this feature, every function definition in a {tech}[mutual block] must be annotated with the {keywordOf Lean.Parser.Command.declaration}`partial_fixpoint` modifier.
+
+```lean (show := false)
+section
+variable (p : Nat → Bool)
+```
 
 :::example "Definition by Partial Fixpoint"
 
-The following function find the least natural number for which the predicate `p` holds.
-If `p` never holds then this equation does not specify the behavior: the function `find` could return 42 in that case, and still satisfy the equation.
+The following function finds the least natural number for which the predicate {lean}`p` holds.
+If `p` never holds, then this equation does not specify the behavior: the function {lean}`find` could return {lean type:="Nat"}`42` or any other {lean}`Nat` in that case and still satisfy the equation.
 
-```lean (keep := false)
+```lean
 def find (p : Nat → Bool) (i : Nat := 0) : Nat :=
   if p i then
     i
@@ -56,42 +72,72 @@ def find (p : Nat → Bool) (i : Nat := 0) : Nat :=
 partial_fixpoint
 ```
 
-The elaborator can prove that functions satisfying the equation exist, and defined `find` to be an arbitrary such function.
+The elaborator can prove that functions satisfying the equation exist.
+Within Lean's logic, {lean}`find` is defined to be an arbitrary such function.
 :::
 
-# Tail-recursive functions
+```lean (show := false)
+end
+```
+
+# Tail-Recursive Functions
 %%%
 tag := "partial-fixpoint-tailrec"
 %%%
 
-Definition by partial fixpoint will succeed if the following two conditions hold:
+:::paragraph
 
-1. The function's type is inhabited (as with {ref "partial-unsafe"}[functions marked {keywordOf Lean.Parser.Command.declaration}`partial`]).
-2. All recursive calls are in {tech}[tail position] of the function.
+A recursive function can be defined as a partial fixpoint if the following two conditions hold:
 
-A {deftech}_tail position_ of the function body is
+ 1. The function's return type is inhabited (as with {ref "partial-unsafe"}[functions marked {keywordOf Lean.Parser.Command.declaration}`partial`]) - either a {name}`Nonempty` or {name}`Inhabited` instance works.
+ 2. All recursive calls are in {tech}[tail position] of the function.
 
-* the function body itself,
-* the branches of a {keywordOf Lean.Parser.Term.match}`match` expression in tail position,
-* the branches of an {keywordOf termIfThenElse}`if` expression in tail position, and
-* the body of a {keywordOf Lean.Parser.Term.let}`let` expression in tail position.
+An expression is in {deftech}_tail position_ in the function body if it is:
 
-In particular, the {tech key:="match discriminant"}[discriminant] of a {keywordOf Lean.Parser.Term.match}`match` expression, the condition of an {keywordOf termIfThenElse}`if` expression and the arguments of functions are not tail-positions.
+ * the function body itself,
+ * the branches of a {keywordOf Lean.Parser.Term.match}`match` expression that is in tail position,
+ * the branches of an {keywordOf termIfThenElse}`if` expression that is in tail position, and
+ * the body of a {keywordOf Lean.Parser.Term.let}`let` expression that is in tail position.
 
-:::example "Tail recursive functions"
+In particular, the {tech key:="match discriminant"}[discriminant] of a {keywordOf Lean.Parser.Term.match}`match` expression, the condition of an {keywordOf termIfThenElse}`if` expression and the arguments of functions are not tail positions.
 
-Because the function body itself is a tail-position, clearly looping definitions are accepted:
+:::
 
-```lean (keep := false)
+```lean (show := false)
+-- Test that nonempty is enough
+inductive A : Type where
+  | mkA
+  | mkA'
+
+instance : Nonempty A := ⟨.mkA⟩
+
+def getA (n : Nat) : A :=
+  getA (n + 1)
+partial_fixpoint
+
+example (n : Nat) : getA n = getA (n + 3) := by
+  conv => lhs; rw [getA, getA, getA]
+```
+
+:::example "Loops are Tail Recursive Functions"
+
+Because the function body itself is a {tech}[tail position], the infinitely looping function {lean}`loop` is tail recursive.
+It can be defined as a partial fixpoint.
+
+```lean
 def loop (x : Nat) : Nat := loop (x + 1)
 partial_fixpoint
 ```
 
-More useful function definitions tend to have some branching.
-The following example could also be constructed using well-founded recursion with a termination proof, but may be more convenient to define using  {keywordOf Lean.Parser.Command.declaration}`partial_fixpoint`, where no termination proof is needed.
+:::
 
-```lean (keep := false)
-def Array.find (xs : Array α) (p : α → Bool) (i : Nat := 0) : Option α :=
+:::example "Tail Recursion with Branching"
+
+{lean}`Array.find` could also be constructed using well-founded recursion with a termination proof, but may be more convenient to define using {keywordOf Lean.Parser.Command.declaration}`partial_fixpoint`, where no termination proof is needed.
+
+```lean
+def Array.find (xs : Array α) (p : α → Bool)
+    (i : Nat := 0) : Option α :=
   if h : i < xs.size then
     if p xs[i] then
       some xs[i]
@@ -116,6 +162,7 @@ def List.findIndex (xs : List α) (p : α → Bool) : Int :=
       if r = -1 then -1 else r + 1
 partial_fixpoint
 ```
+The error message on the recursive call is:
 ```leanOutput nonTailPos
 Could not prove 'List.findIndex' to be monotone in its recursive calls:
   Cannot eliminate recursive call `List.findIndex ys p` enclosed in
@@ -131,11 +178,11 @@ tag := "partial-fixpoint-monadic"
 %%%
 
 
-Definition by partial fixpoint is more powerful if the function's type is monadic and the monad is an instance of {name}`Lean.Order.MonoBind`, such as {name}`Option`.
-In this case, recursive call are not restricted to tail-positions, but can also be inside higher-order monadic functions such as {name}`bind` and {name}`List.mapM`.
+Defining a function as a partial fixpoint is more powerful if the function's return type is a monad that is an instance of {name}`Lean.Order.MonoBind`, such as {name}`Option`.
+In this case, recursive call are not restricted to tail-positions, but may also occur inside higher-order monadic functions such as {name}`bind` and {name}`List.mapM`.
 
 The set of higher-order functions for which this works is extensible (see TODO below), so no exhaustive list is given here.
-The aspiration is that a monadic recursive function definition that is built using abstract monadic operations like {name}`bind`, but not open the abstraction of the monad (e.g. by matching on the {name}`Option` value), is accepted.
+The aspiration is that a monadic recursive function definition that is built using abstract monadic operations like {name}`bind`, but that does not open the abstraction of the monad (e.g. by matching on the {name}`Option` value), is accepted.
 In particular, using {tech}[{keywordOf Lean.Parser.Term.do}`do`-notation] should work.
 
 :::example "Monadic functions"
@@ -167,7 +214,7 @@ def Tree.rev' (t : Tree) : Option Tree := do
 partial_fixpoint
 ```
 
-Pattern matching on the result of the recursive call will prevent the definition by partial fixpoint to go through:
+Pattern matching on the result of the recursive call will prevent the definition by partial fixpoint from going through:
 
 ```lean (keep := false) (error := true) (name := monoMatch)
 def List.findIndex (xs : List α) (p : α → Bool) : Option Nat :=
@@ -190,7 +237,7 @@ Could not prove 'List.findIndex' to be monotone in its recursive calls:
     | some r => some (r + 1)
 ```
 
-In this particular case, using the {name}`Functor.map` function instead of explicit pattern matching helps:
+In this particular case, using {name}`Functor.map` instead of explicit pattern matching helps:
 
 ```lean
 def List.findIndex (xs : List α) (p : α → Bool) : Option Nat :=
@@ -205,21 +252,25 @@ partial_fixpoint
 ```
 :::
 
-# Partial Correctness Theorem
+# Partial Correctness Theorems
 %%%
 tag := "partial-correctness-theorem"
 %%%
 
-In general, for functions defined by partial fixpoint we only obtain the equational theorems that prove that the function indeed satisfies the given equation, and enables proofs by rewriting.
-But these do not allow reasoning about the behavior of the function on arguments for which the function specification does not terminate.
 
-If the monad happens to be the {name}`Option` monad, then by construction the function equals {name}`Option.none` on all function inputs for which the defining equation is not terminating.
-From this fact, Lean proves a {deftech}_partial correctness theorem_ for the function which allows concluding facts from the function's result being {name}`Option.some`.
+For every function defined as a partial fixpoint, Lean proves that that the defining equation is satisfied.
+This enables proofs by rewriting.
+However, these equational theorems are not sufficient for reasoning about the behavior of the function on arguments for which the function specification does not terminate.
+Code paths that lead to infinite recursion at runtime would end up as infinite chains of rewrites in a potential proof.
+
+Partial fixpoints in suitable monads, on the other hand, provide additional theorems that map the undefined values from non-termination to suitable values in the monad.
+In the {name}`Option` monad, then partial fixpoint equals {name}`Option.none` on all function inputs for which the defining equation specifies non-termination.
+From this fact, Lean proves a {deftech}_partial correctness theorem_ for the function which allows facts to be concluded when the function's result is {name}`Option.some`.
 
 
-:::example "Partial correctness theorem"
+::::example "Partial Correctness Theorem"
 
-Recall this function from an earlier example:
+Recall {lean}`List.findIndex` from an earlier example:
 
 ```lean
 def List.findIndex (xs : List α) (p : α → Bool) : Option Nat :=
@@ -233,11 +284,9 @@ def List.findIndex (xs : List α) (p : α → Bool) : Option Nat :=
 partial_fixpoint
 ```
 
-With this function definition, Lean proves the following partial correctness theorem:
+With this function definition, Lean automatically proves the following partial correctness theorem:
 
-{TODO}[using `signature` causes max recursion error]
-
-```
+```signature
 List.findIndex.partial_correctness {α : Type _} (motive : List α → (α → Bool) → Nat → Prop)
   (h :
     ∀ (findIndex : List α → (α → Bool) → Option Nat),
@@ -251,13 +300,26 @@ List.findIndex.partial_correctness {α : Type _} (motive : List α → (α → B
   (xs : List α) (p : α → Bool) (r : Nat) : xs.findIndex p = some r → motive xs p r
 ```
 
-We can use this theorem to prove that the resulting number is a valid index in the list and that the predicate holds for that index:
+:::paragraph
+Here, the motive is a relation between the parameter and return types of {lean}`List.findIndex`, with the {name}`Option` removed from the return type.
+If, when given an arbitrary partial function with a signature that's compatible with {lean}`List.findIndex`, the following hold:
+
+ * the motive is satisfied for all inputs for which the arbitrary function returns a value (rather than {name}`none`),
+
+ * taking one rewriting step with the defining equation, in which the recursive calls are replaced by the arbitrary function, also implies the satisfaction of the motive
+
+then the motive is satsified for all inputs for which the {lean}`List.findIndex` returns {name}`some`.
+
+:::
+
+The partial correctness theorem is a reasoning principle.
+It can be used to prove that the resulting number is a valid index in the list and that the predicate holds for that index:
 
 ```lean
 theorem List.findIndex_implies_pred (xs : List α) (p : α → Bool) :
-    xs.findIndex p = some i → xs[i]?.any p := by
+    xs.findIndex p = some i → ∃x, xs[i]? = some x ∧ p x := by
   apply List.findIndex.partial_correctness
-          (motive := fun xs p i => xs[i]?.any p)
+          (motive := fun xs p i => ∃ x, xs[i]? = some x ∧ p x)
   intro findIndex ih xs p r hsome
   split at hsome
   next => contradiction
@@ -273,9 +335,9 @@ theorem List.findIndex_implies_pred (xs : List α) (p : α → Bool) :
       simpa
 ```
 
-:::
+::::
 
-# Mutual Well-Founded Recursion
+# Mutual Recursion with Partial Fixpoints
 %%%
 tag := "mutual-partial-fixpoint"
 %%%
@@ -295,14 +357,25 @@ The construction builds on a variant of the Knaster–Tarski theorem: In a chain
 
 The necessary theory is found in the `Lean.Order` namespace.
 This is not meant to be a general purpose library of order theoretic results.
-Instead, the definitions and theorems therein are only intended to back the
-{keywordOf Lean.Parser.Command.declaration}`partial_fixpoint` feature.
+Instead, the definitions and theorems in `Lean.Order` are only intended as implementation details of the {keywordOf Lean.Parser.Command.declaration}`partial_fixpoint` feature, and they should be considered a private API that may change without notice.
 
-The notion of a partial order, and that of a chain-complete partial order, are represented as type classes:
+The notion of a partial order, and that of a chain-complete partial order, are represented by the type classes {name}`Lean.Order.PartialOrder` and {name}`Lean.Order.CCPO`, respectively.
 
 {docstring Lean.Order.PartialOrder}
 
 {docstring Lean.Order.CCPO}
+
+```lean (show := false)
+section
+open Lean.Order
+variable {α : Type u} {β : Type v} [PartialOrder α] [PartialOrder β] (f : α → β) (x y : α)
+```
+
+A function is monotone if it preserves partial orders.
+That is, if {lean}`x ⊑ y` then {lean}`f x ⊑ f y`.
+The operator `⊑` represent {name}`Lean.Order.PartialOrder.rel`.
+
+{docstring Lean.Order.monotone}
 
 The fixpoint of a monotone function can be taken using {name}`fix`, which indeed constructs a fixpoint, as shown by {name}`fix_eq`,
 
@@ -310,7 +383,9 @@ The fixpoint of a monotone function can be taken using {name}`fix`, which indeed
 
 {docstring Lean.Order.fix_eq}
 
-So to construct the function, Lean first infers a suitable {name}`CCPO` instance.
+:::paragraph
+
+To construct the partial fixpoint, Lean first synthesizes a suitable {name}`CCPO` instance.
 
 ```lean (show := false)
 section
@@ -322,13 +397,15 @@ variable (w : α)
 
 * If the function's result type has a dedicated instance, like {name}`Option` has with {name}`instCCPOOption`, this is used together with the instance for the function type, {name}`instCCPOPi`, to construct an instance for the whole function's type.
 
-* Else, if the function's type can be shown to be inhabited by a witness {lean}`w`, then the instance {name}`FlatOrder.instCCPO` for the wrapper type {lean}`FlatOrder w` is used. In this order, {lean}`w` is a least element and all other elements are incomparable.
+* Otherwise, if the function's type can be shown to be inhabited by a witness {lean}`w`, then the instance {name}`FlatOrder.instCCPO` for the wrapper type {lean}`FlatOrder w` is used. In this order, {lean}`w` is a least element and all other elements are incomparable.
 
 ```lean (show := false)
 end
 ```
 
-Next, the recursive calls in the right-hand side of the function definitions are abstracted; this turns into the argument `f` of {name}`fix`. The monotonicity requirement is solved by the {tactic}`monotonicity` tactic, which applies compositional monotonicity lemmas in a syntax-driven way
+:::
+
+Next, the recursive calls in the right-hand side of the function definitions are abstracted; this turns into the argument `f` of {name}`fix`. The monotonicity requirement is solved by the {tactic}`monotonicity` tactic, which applies compositional monotonicity lemmas in a syntax-driven way.
 
 ```lean (show := false)
 section
